State proposition 18

Authentication_Tests.v
@@ -1,10 +1,6 @@
 
 Require Import Strand_Spaces Strand_Library Message_Algebra Authentication_Tests_Library.
 
-Definition not_proper_subterm (t:msg) :=  
-  exists (n': node) (L : msg), 
-  t <st L -> t <> L -> r_node n' -> L <[node] n' -> False.
-
 Definition test_component (a t: msg) (n:node) : Prop :=
   (exists h k, t = E h k) /\ a <st t /\ t <[node] n /\ not_proper_subterm t.
 
@@ -22,14 +18,18 @@ Variable n n' : node.
 Variable a t: msg.
 Hypothesis incom : incoming_test n n' a t.
 
-Theorem Authentication_test2 : 
-  incoming_test n n' a t ->
-  exists m m', r_node m /\ r_node m' /\ t <[node] m /\
-  transforming_edge_for m m' a.
-Admitted.
 Theorem Authentication_test1 :
   outgoing_test n n' a t ->
   exists m m', r_node m /\ r_node m' /\ t <[node] m' /\
   transforming_edge_for m m' a.
 Admitted.
+
+Theorem Authentication_test2 : 
+  incoming_test n n' a t ->
+  exists m m', r_node m /\ r_node m' /\ t <[node] m /\
+  transforming_edge_for m m' a.
+Proof.
+intros.
+Admitted.
+
 End Authentication_tests.  
